src/Expr.v
@@ -1069,6 +1069,16 @@ Section env.
       induction a; simpl; try solve [ intuition auto ]; intros.
     Qed.
     
+    Lemma AllProvable_impl_AllProvable : forall P ps,
+      AllProvable ps ->
+      AllProvable_impl P ps ->
+      P.
+    Proof. clear. induction ps; simpl; intros; eauto. intuition. Qed.
+
+    Lemma AllProvable_and_sem : forall P Ps,
+      AllProvable_and P Ps <-> (AllProvable Ps /\ P).
+    Proof. induction Ps; simpl; intros; intuition auto. Qed.
+    
     Lemma Provable_ValidProp : forall goal, Provable goal -> ValidProp goal.
       unfold Provable, ValidProp in *; intros;
         repeat match goal with
