src/UnfolderTac.v
@@ -1,0 +1,310 @@
+Require Import List Bool.
+Require Import Expr SepExpr.
+Require Import Prover.
+Require Import Tactics Reflection.
+Require Unfolder.
+Require SepHeap.
+
+Set Implicit Arguments.
+Set Strict Implicit.
+
+Module UnfolderTac (UNF : Unfolder.Unfolder).
+  Module SH_UTIL := SepHeap.SepHeapFacts UNF.SH.
+  Module SE_EXT := SepExpr.SepExprFacts UNF.SH.SE.
+
+Section unfolder.
+  Variable types : list type.
+  Variable funcs : functions types.
+  Variable preds : UNF.SH.SE.predicates types.
+  Variable prover : ProverT types.
+  Variable facts : Facts prover.
+  Variable hintsFwd : option (UNF.hintSide types).
+  Variable hintsBwd : option (UNF.hintSide types).
+
+  Record unfolderResult : Type :=
+  { Alls : list tvar
+  ; Exs  : list tvar
+  ; Lhs  : UNF.SH.SHeap types
+  ; Rhs  : UNF.SH.SHeap types
+  }.
+
+  Definition unfold (uvars : list tvar)
+    (ql : list tvar) (lhs rhs : UNF.SH.SHeap types) : unfolderResult * bool :=
+    let pre :=
+      {| UNF.Vars  := ql
+       ; UNF.UVars := uvars
+       ; UNF.Heap  := lhs
+      |}
+    in
+    match match hintsFwd with
+            | None => (pre, false)
+            | Some hints => UNF.refineForward prover hints 10 facts pre 
+          end
+      with
+      | ({| UNF.Vars := vars' ; UNF.UVars := uvars' ; UNF.Heap := lhs |}, fprog) =>
+        let post :=
+          {| UNF.Vars  := vars'
+           ; UNF.UVars := uvars'
+           ; UNF.Heap  := rhs
+          |}
+        in
+        match match hintsBwd with
+                | None => (post, false)
+                | Some hints => 
+                  let facts' := Learn _ facts (UNF.SH.pures lhs) in
+                  UNF.refineBackward prover hints 10 facts' post
+              end
+        with
+          | ({| UNF.Vars := vars' ; UNF.UVars := uvars' ; UNF.Heap := rhs |}, bprog) =>
+            let new_vars  := skipn (length ql) vars' in
+            let new_uvars := skipn (length uvars) uvars' in
+            let bound := length uvars' in
+            ({| Alls := new_vars
+              ; Exs  := new_uvars
+              ; Lhs  := lhs
+              ; Rhs  := rhs
+              |}, fprog || bprog)
+        end
+    end.
+
+  Lemma WellTyped_env_app : forall ts a b c d,
+    WellTyped_env a c ->
+    WellTyped_env b d ->
+    WellTyped_env (types := ts) (a ++ b) (c ++ d).
+  Proof. clear.
+    intros. unfold WellTyped_env in *. unfold typeof_env in *. subst. 
+    rewrite map_app. reflexivity.
+  Qed.
+  Ltac t_list_length := repeat (rewrite typeof_env_length || rewrite rev_length || rewrite map_length || rewrite app_length).
+  Hint Extern 1 (_ = _) => t_list_length; auto : list_length.
+
+  Ltac env_resolution :=
+    repeat (rewrite typeof_env_app || unfold typeof_env || rewrite map_app || rewrite map_rev || (f_equal; []) || assumption).
+
+  Hypothesis prover_Correct : ProverT_correct prover funcs.
+  Hypothesis hintsFwd_Correct : match hintsFwd with
+                                  | Some hints => UNF.hintSideD funcs preds hints
+                                  | None => True
+                                end.
+  Hypothesis hintsBwd_Correct : match hintsBwd with
+                                  | Some hints => UNF.hintSideD funcs preds hints
+                                  | None => True
+                                end.
+
+  Lemma ApplyUnfold_with_eq' : 
+    forall (var_env meta_env : env types),
+    Valid prover_Correct meta_env var_env facts ->
+    forall (l r : UNF.SH.SHeap types) res,
+    forall (WTR : UNF.SH.WellTyped_sheap (typeof_funcs funcs) (UNF.SH.SE.typeof_preds preds) (typeof_env meta_env) (typeof_env var_env) r = true) b,
+    unfold (typeof_env meta_env) (typeof_env var_env) l r = (res, b) ->
+    match res with
+      | {| Alls := new_vars
+         ; Exs  := new_uvars
+         ; Lhs  := lhs'
+         ; Rhs  := rhs'
+         |} =>
+        Expr.forallEach new_vars (fun nvs : Expr.env types =>
+          let var_env := var_env ++ nvs in
+          Expr.AllProvable_impl funcs meta_env var_env
+          (Expr.existsEach new_uvars (fun menv : Expr.env types =>
+            let meta_env := meta_env ++ menv in
+                (Expr.AllProvable_and funcs meta_env var_env
+                  (UNF.SH.SE.ST.himp
+                    (UNF.SH.SE.sexprD funcs preds meta_env var_env
+                      (UNF.SH.sheapD (UNF.SH.Build_SHeap (UNF.SH.impures lhs') nil (UNF.SH.other lhs'))))
+                    (UNF.SH.SE.sexprD funcs preds meta_env var_env
+                      (UNF.SH.sheapD (UNF.SH.Build_SHeap (UNF.SH.impures rhs') nil (UNF.SH.other rhs')))))
+                  (UNF.SH.pures rhs')) ))
+            (UNF.SH.pures lhs'))
+    end ->
+    UNF.SH.SE.ST.himp (@UNF.SH.SE.sexprD _ funcs preds meta_env var_env (UNF.SH.sheapD l))
+                      (@UNF.SH.SE.sexprD _ funcs preds meta_env var_env (UNF.SH.sheapD r)).
+  Proof.
+    Opaque Env.repr.
+    intros. unfold unfold in *.
+    destruct res.
+
+    match goal with
+      | [ H : match ?X with _ => _ end = _ |- _ ] => consider X
+    end; intros.
+    destruct u.
+    match goal with
+      | [ H : match ?X with _ => _ end = _ |- _ ] => consider X
+    end; intros.
+    destruct u.
+    inversion H3; clear H3. subst Heap Heap0 b.
+
+    eapply SH_UTIL.SEP_FACTS.himp_WellTyped_sexpr; intros.
+
+    assert (UVars = typeof_env meta_env /\ 
+      typeof_env var_env = firstn (length var_env) Vars /\
+    UNF.SH.SE.ST.himp 
+      (UNF.SH.SE.sexprD funcs preds meta_env var_env (UNF.SH.sheapD l))
+      (UNF.ST_EXT.existsEach (skipn (length var_env) Vars)
+        (fun vars_ext : list {t : tvar & tvarD types t} =>
+          UNF.SH.SE.sexprD funcs preds meta_env 
+          (var_env ++ vars_ext) (UNF.SH.sheapD Lhs0)))).
+    { clear H2 H1. destruct hintsFwd. 
+      { generalize (UNF.refineForward_Length H0).
+        eapply UNF.refineForward_Ok in H0; eauto using typeof_env_WellTyped_env.
+        intro. destruct H1. destruct H1. simpl in *. split; auto. split; auto.
+        subst.
+        rewrite ListFacts.firstn_app_exact; auto. unfold typeof_env. rewrite map_length. auto.
+        simpl; rewrite UNF.SH.WellTyped_sheap_WellTyped_sexpr; eassumption. }
+      { inversion H0; clear H0; subst. split; auto.
+        split. rewrite <- app_nil_r with (l := typeof_env var_env).
+        rewrite ListFacts.firstn_app_exact. rewrite app_nil_r. auto. unfold typeof_env. rewrite map_length; auto.
+        unfold typeof_env.
+        erewrite ListFacts.skipn_length_all by reflexivity.
+        rewrite UNF.ST_EXT.existsEach_nil. rewrite app_nil_r. reflexivity. } }
+    destruct H4. destruct H7. rewrite H8; clear H8.
+    rewrite UNF.ST_EXT.himp_existsEach_p; [ reflexivity | intros ].
+
+    destruct hintsBwd.
+    { assert (Vars = typeof_env var_env ++ skipn (length var_env) Vars); intros.
+      rewrite <- firstn_skipn with (n := length var_env) (l := Vars) at 1.
+      rewrite <- H8. rewrite H7. reflexivity.
+
+      generalize (UNF.refineBackward_Length H2); intros.
+      destruct H10; simpl in *. destruct H10. subst Vars0.
+
+      apply SH_UTIL.himp_pull_pures; intros.
+
+      eapply UNF.refineBackward_Ok in H2.
+      2: eassumption.
+      2: eassumption.
+      Focus 2. simpl. rewrite H4. eapply typeof_env_WellTyped_env.
+      Focus 2. simpl. instantiate (1 := var_env ++ G). unfold WellTyped_env, typeof_env.
+      rewrite map_app. rewrite H9. rewrite <- H8. reflexivity.
+
+      Focus 2. simpl. rewrite H9; clear H9. subst; simpl.
+      clear - WTR.
+      repeat rewrite UNF.SH.WellTyped_sheap_WellTyped_sexpr in *.
+      eapply SH_UTIL.SEP_FACTS.WellTyped_sexpr_weaken with (U' := nil) in WTR. rewrite app_nil_r in WTR. eauto.
+      
+      { simpl in *.
+        rewrite SH_UTIL.SEP_FACTS.sexprD_weaken_wt with (U' := nil) (G' := G) (s := UNF.SH.sheapD r).
+        rewrite app_nil_r.
+        rewrite <- H2; clear H2. subst UVars0 Alls0.
+        eapply forallEach_sem in H1.
+        Focus 2.
+        unfold typeof_env in *. rewrite map_length. eassumption.
+        apply SH_UTIL.himp_pull_pures; intro.
+        eapply AllProvable_impl_AllProvable in H1; eauto.
+        eapply existsEach_sem in H1. destruct H1. destruct H1.
+        eapply AllProvable_and_sem in H5. destruct H5.
+        eapply SH_UTIL.sheapD_remove_pures_p. 
+        eapply UNF.ST_EXT.himp_existsEach_c. exists x0. split. subst UVars Exs0.
+        unfold typeof_env in *.
+        rewrite <- H6. rewrite map_length. reflexivity.
+
+        eapply SH_UTIL.sheapD_remove_pures_c; eauto. rewrite <- H11; clear H11.
+
+        eapply SH_UTIL.SEP_FACTS.himp_WellTyped_sexpr; intros.
+        rewrite SH_UTIL.SEP_FACTS.sexprD_weaken_wt with (U' := x0) (G' := nil) by eassumption.
+        rewrite app_nil_r. reflexivity.  
+
+        rewrite <- UNF.SH.WellTyped_sheap_WellTyped_sexpr. eassumption. }
+
+      eapply Valid_weaken with (ue := nil) (ge := G) in H.
+      rewrite app_nil_r in *; eauto.
+      eapply Learn_correct; eassumption. }
+    { inversion H2; clear H2; subst.
+      eapply forallEach_sem in H1. 
+      2: unfold typeof_env; rewrite map_length; eassumption.
+      apply SH_UTIL.himp_pull_pures; intro.
+      eapply AllProvable_impl_AllProvable in H1; eauto.
+      apply existsEach_sem in H1. destruct H1. destruct H1.
+      eapply AllProvable_and_sem in H4. destruct H4.
+
+      rewrite SH_UTIL.SEP_FACTS.sexprD_weaken_wt with (U' := x) (G' := G) (s := UNF.SH.sheapD Rhs0).
+      2: rewrite <- UNF.SH.WellTyped_sheap_WellTyped_sexpr; eassumption.
+
+      eapply SH_UTIL.SEP_FACTS.himp_WellTyped_sexpr; intros.
+      rewrite SH_UTIL.SEP_FACTS.sexprD_weaken_wt with (U' := x) (G' := nil) (s := UNF.SH.sheapD Lhs0) by eassumption.
+      clear H7.
+      rewrite app_nil_r.
+
+      eapply SH_UTIL.sheapD_remove_pures_p.
+      eapply SH_UTIL.sheapD_remove_pures_c; eauto. } 
+  Qed.
+
+(*
+  Lemma ApplyCancelSep_with_eq : 
+    forall (algos_correct : ILAlgoTypes.AllAlgos_correct funcs preds algos),
+    forall (meta_env : env (Env.repr BedrockCoreEnv.core types)) (hyps : Expr.exprs (_)),
+
+    forall (l r : SEP.sexpr types BedrockCoreEnv.pc BedrockCoreEnv.st) res,
+    unfolder (typeof_env meta_env) hyps l r = Some res ->
+    Expr.AllProvable funcs meta_env nil hyps ->
+    forall (WTR : SEP.WellTyped_sexpr (typeof_funcs funcs) (SEP.typeof_preds preds) (typeof_env meta_env) nil r = true) cs,
+
+    match res with
+      | {| AllExt := new_vars
+         ; ExExt  := new_uvars
+         ; Lhs    := lhs'
+         ; Rhs    := rhs'
+         ; Subst  := subst
+         |} =>
+        Expr.forallEach new_vars (fun nvs : Expr.env types =>
+          let var_env := nvs in
+          Expr.AllProvable_impl funcs meta_env var_env
+          (existsSubst funcs var_env subst 0 
+            (map (fun x => existT (fun t => option (tvarD types t)) (projT1 x) (Some (projT2 x))) meta_env ++
+             map (fun x => existT (fun t => option (tvarD types t)) x None) new_uvars)
+            (fun meta_env : Expr.env types =>
+                (Expr.AllProvable_and funcs meta_env var_env
+                  (himp cs 
+                    (SEP.sexprD funcs preds meta_env var_env
+                      (SH.sheapD (SH.Build_SHeap _ _ (SH.impures lhs') nil (SH.other lhs'))))
+                    (SEP.sexprD funcs preds meta_env var_env
+                      (SH.sheapD (SH.Build_SHeap _ _ (SH.impures rhs') nil (SH.other rhs')))))
+                  (SH.pures rhs')) ))
+            (SH.pures lhs'))
+    end ->
+    himp cs (@SEP.sexprD _ _ _ funcs preds meta_env nil l)
+            (@SEP.sexprD _ _ _ funcs preds meta_env nil r).
+  Proof. intros. eapply ApplyCancelSep_with_eq'; eauto. Qed.
+
+  Lemma ApplyCancelSep : 
+    forall (algos_correct : ILAlgoTypes.AllAlgos_correct funcs preds algos),
+    forall (meta_env : env (Env.repr BedrockCoreEnv.core types)) (hyps : Expr.exprs (_)),
+    forall (l r : SEP.sexpr types BedrockCoreEnv.pc BedrockCoreEnv.st),
+      Expr.AllProvable funcs meta_env nil hyps ->
+    forall (WTR : SEP.WellTyped_sexpr (typeof_funcs funcs) (SEP.typeof_preds preds) (typeof_env meta_env) nil r = true) cs,
+    match unfolder (typeof_env meta_env) hyps l r with
+      | Some {| AllExt := new_vars
+         ; ExExt  := new_uvars
+         ; Lhs    := lhs'
+         ; Rhs    := rhs'
+         ; Subst  := subst
+         |} =>
+        Expr.forallEach new_vars (fun nvs : Expr.env types =>
+          let var_env := nvs in
+          Expr.AllProvable_impl funcs meta_env var_env
+          (existsSubst funcs var_env subst 0 
+            (map (fun x => existT (fun t => option (tvarD types t)) (projT1 x) (Some (projT2 x))) meta_env ++
+             map (fun x => existT (fun t => option (tvarD types t)) x None) new_uvars)
+            (fun meta_env : Expr.env types =>
+                (Expr.AllProvable_and funcs meta_env var_env
+                  (himp cs 
+                    (SEP.sexprD funcs preds meta_env var_env
+                      (SH.sheapD (SH.Build_SHeap _ _ (SH.impures lhs') nil (SH.other lhs'))))
+                    (SEP.sexprD funcs preds meta_env var_env
+                      (SH.sheapD (SH.Build_SHeap _ _ (SH.impures rhs') nil (SH.other rhs')))))
+                  (SH.pures rhs')) ))
+            (SH.pures lhs'))
+      | None => 
+        himp cs (@SEP.sexprD _ _ _ funcs preds meta_env nil l)
+                (@SEP.sexprD _ _ _ funcs preds meta_env nil r)
+    end ->
+    himp cs (@SEP.sexprD _ _ _ funcs preds meta_env nil l)
+            (@SEP.sexprD _ _ _ funcs preds meta_env nil r).
+  Proof. 
+    intros. consider (unfolder (typeof_env meta_env) hyps l r); intros; auto.
+    eapply ApplyCancelSep_with_eq; eauto.
+  Qed.
+*)
+
+End unfolder.
+End UnfolderTac.
